add uint8 loop

src/callMain.c
@@ -1,0 +1,27 @@
+#include <stdio.h>
+#include <stdlib.h>
+
+#include "Main.h"
+
+int main(int argc, char *argv[]) {
+    FILE *fp;
+    char *fname = "publishMessagePacket.bin";
+    uint8_t request[10000];
+    uint32_t  i;
+    uint32_t size;
+
+    fp = fopen( fname, "rb" );
+    if( fp == NULL ){
+    printf( "%sファイルが開けません", fname );
+    return -1;
+    }
+
+    size = fread( request, sizeof( unsigned char ), 10000, fp );
+    fclose(fp);
+    // for(i=0; i<size; i++ ){
+    //     printf("%02x\n", request[i]);
+    // }
+    
+    parse(request, size);
+    return 0;
+}
