src/main.fst
@@ -1,11 +1,44 @@
 module Main
 
-open FStar.HyperStack.ST
-module LP = LowStar.Printf
+module B = LowStar.Buffer
+module M = LowStar.Modifies
+module U32 = FStar.UInt32
 
-val main : u:unit -> Stack C.exit_code (fun _ -> True) (fun _ _ _ -> True)
-let main () =
+open FStar.HyperStack.ST
+open LowStar.BufferOps
+open LowStar.Printf
+
+module HS = FStar.HyperStack
+module ST = FStar.HyperStack.ST
+module U32 = FStar.UInt32
+module U8 = FStar.UInt8
+
+val normal_loop: src:B.buffer U8.t -> len:U32.t -> Stack C.exit_code
+  (requires fun h0 -> B.live h0 src /\ B.length src = U32.v len )
+  (ensures fun _ _ _ -> true)
+let normal_loop src len =
+  let inv h (i: nat) = B.live h src in
+  let body (i: U32.t{ 0 <= U32.v i /\ U32.v i < U32.v len }): Stack unit
+    (requires (fun h -> inv h (U32.v i)))
+    (ensures (fun _ _ _ -> true))
+  =
+    let v : U8.t = src.(i) in
+    print_u8 v;
+    print_string "\n" // TODO: 後で消す
+  in
+  C.Loops.for 0ul len inv body;
+  (* return *) C.EXIT_SUCCESS
+
+val parse (request: B.buffer U8.t) (len: U32.t):
+  Stack C.exit_code 
+    (requires (fun h ->
+      B.live h request /\
+      B.length request = U32.v len  ))
+    (ensures (fun h0 _ h1 ->
+      B.live h1 request))
+
+let parse request len =
     push_frame ();
-    LP.print_string "Hello verimqtt.\n";
+    let r = normal_loop request len in
     pop_frame ();
     C.EXIT_SUCCESS
